wip basic blocks verification

src/verification/BlockVer/Examples.v
@@ -25,44 +25,25 @@ Import bv.notations.
 Import env.notations.
 Import ListNotations.
 Import asn.notations.
+Import Erasure.notations.
 
 Module Examples.
-  Definition asn_mpu_registers {Σ} : Assertion Σ :=
-      ∃ "MPUCTL0_reg"    , MPUCTL0_reg    ↦ term_var "MPUCTL0_reg"
-    ∗ ∃ "MPUCTL1_reg"    , MPUCTL1_reg    ↦ term_var "MPUCTL1_reg"
-    ∗ ∃ "MPUSEGB2_reg"   , MPUSEGB2_reg   ↦ term_var "MPUSEGB2_reg"
-    ∗ ∃ "MPUSEGB1_reg"   , MPUSEGB1_reg   ↦ term_var "MPUSEGB1_reg"
-    ∗ ∃ "MPUSAM_reg"     , MPUSAM_reg     ↦ term_var "MPUSAM_reg".
+  Import Utils.
 
-  Definition minimal_pre {Σ} : Assertion Σ :=
-    ∃ "ipectl", MPUIPC0_reg    ↦ term_var "ipectl" ∗
-    ∃ "segb1" , MPUIPSEGB1_reg ↦ term_var "segb1"  ∗
-    ∃ "segb2" , MPUIPSEGB2_reg ↦ term_var "segb2"  ∗
-    asn_mpu_registers.
+  Definition asn_ipe_registers {Σ} : Assertion Σ :=
+      ∃ "ipectl", MPUIPC0_reg          ↦ term_var "ipectl"
+    ∗ ∃ "segb1" , MPUIPSEGB1_reg       ↦ term_var "segb1"
+    ∗ ∃ "segb2" , MPUIPSEGB2_reg       ↦ term_var "segb2".
 
-  Definition minimal_post {Σ} : Assertion Σ := minimal_pre.
+  Definition minimal_pre {Σ} (include_ipe : bool) : Assertion Σ :=
+      ∃ "lif", LastInstructionFetch ↦ term_var "lif"
+    ∗ ∃ "srcg1", SRCG1_reg ↦ term_var "srcg1"
+    ∗ if include_ipe then asn_ipe_registers else ⊤
+    ∗ asn_mpu_registers.
 
-  Definition VC_triple {Σ}
-    (P : Assertion (Σ ▻ "a" :: ty.wordBits))
-    (i : list ast_with_args)
-    (Q : Assertion (Σ ▻ "a" :: ty.wordBits ▻ "an" :: ty.wordBits))
-  :=
-    sblock_verification_condition
-      (minimal_pre ∗ P) i (minimal_post ∗ Q) wnil.
 
-  Definition Valid_VC {Σ}
-    (P : Assertion (Σ ▻ "a" :: ty.Address))
-    (i : list ast_with_args)
-    (Q : Assertion (Σ ▻ "a" :: ty.Address ▻ "an" :: ty.Address))
-  :=
-    safeE (postprocess (VC_triple P i Q)).
-
-  Definition Debug_VC {Σ}
-    (P : Assertion (Σ ▻ "a" :: ty.Address))
-    (i : list ast_with_args)
-    (Q : Assertion (Σ ▻ "a" :: ty.Address ▻ "an" :: ty.Address))
-  :=
-    VerificationCondition (postprocess (VC_triple P i Q)).
+  Definition minimal_post {Σ} (include_ipe : bool) : Assertion Σ :=
+    minimal_pre include_ipe.
 
   Record BlockVerifierContract {Σ} :=
     MkBlockVerifierContract
@@ -71,38 +52,47 @@ Module Examples.
       ; postcondition : Assertion (Σ ▻ "a" :: ty.Address ▻ "an" :: ty.Address)
       }.
 
-  Definition map {Σ A} (c : @BlockVerifierContract Σ)
-    (f : Assertion (Σ ▻ "a" :: ty.Address) -> list ast_with_args -> Assertion (Σ ▻ "a" :: ty.Address ▻ "an" :: ty.Address) -> A)
-    : A :=
-    match c with
-    | {| precondition := pre; instrs := i; postcondition := post |} =>
-        f pre i post
-    end.
+  Definition MkValidBlockVerifierContract {Σ} (include_ipe : bool) (c : @BlockVerifierContract Σ) : Prop :=
+  match c with
+    {| precondition := pre; instrs := i; postcondition := post |} =>
+      safeE (* VerificationCondition *) (postprocess
+               (sblock_verification_condition
+                  (minimal_pre include_ipe ∗ pre)
+                  i
+                  (minimal_post include_ipe ∗ post)
+                  wnil))
+  end.
 
-  Definition ValidBlockVerifierContract {Σ} (c : @BlockVerifierContract Σ) : Prop :=
-    map c Valid_VC.
+  Definition ValidBlockVerifierContract {Σ} := @MkValidBlockVerifierContract Σ true.
+  Definition ValidBlockVerifierContractWithExplicitIPE {Σ} := @MkValidBlockVerifierContract Σ false.
 
   Local Notation "'{{' P '}}' i '{{' Q '}}'" :=
     (@MkBlockVerifierContract [ctx] P%asn i Q%asn)
       (at level 90, format "'[v' '{{'  P  '}}' '/'  i '/' '{{'  Q  '}}' ']'").
+  Local Notation "'{{' P '}}' i '{{' Q '}}' 'with' logvars" :=
+    (@MkBlockVerifierContract logvars P%asn i Q%asn)
+      (at level 90, format "'[v' '{{'  P  '}}' '/'  i '/' '{{'  Q  '}}' '/' 'with'  logvars ']'").
 
   Local Ltac solve_bv :=
       repeat match goal with
-        | |- context[bv.add ?x (@BitvectorBase.bv.mk ?n 0 I)] =>
+        | |- context[bv.add ?x (@bv.mk ?n 0 I)] =>
             fold (@bv.zero n)
         | |- context[bv.add ?x bv.zero] =>
-            rewrite BitvectorBase.bv.add_zero_r
+            rewrite bv.add_zero_r
         end.
 
-  Local Ltac solve_vc :=
-    vm_compute; constructor; cbn; intros; repeat split; try solve_bv; auto.
+  Local Ltac symbolic_simpl :=
+    vm_compute; constructor; simpl.
 
-  Definition asn_init_pc {Σ} : Assertion (Σ ▻ "a" :: ty.Address) :=
-    term_var "a" = term_val ty.Address bv.zero.
+  Definition asn_init_pc {Σ} (pc : Term _ ty.Address) : Assertion (Σ ▻ "a" :: ty.Address) :=
+    term_var "a" = pc.
+  Definition asn_fin_pc {Σ} (pc : Term _ ty.Address) : Assertion (Σ ▻ "an" :: ty.Address) :=
+    term_var "an" = pc.
 
   Definition ex_mov_register : BlockVerifierContract :=
     {{
-        asn_init_pc ∗
+        asn_init_pc (term_val ty.Address [bv 0]) ∗
+        asn_ipe_registers ∗
         R4_reg ↦ term_val ty.wordBits [bv 42] ∗
         ∃ "v", R5_reg ↦ term_var "v"
     }}
@@ -110,14 +100,435 @@ Module Examples.
     [mov_rr R4 R5]
 
     {{
+        asn_ipe_registers ∗
         R4_reg ↦ term_val ty.wordBits [bv 42] ∗
         R5_reg ↦ term_val ty.wordBits [bv 42]
     }}.
 
+
   Example valid_ex_move_register : ValidBlockVerifierContract ex_mov_register.
-  Proof.
-    solve_vc.
+  Proof. now symbolic_simpl. Qed.
 
-  Qed.
 
+(* { valid sig \/ saved }
+   bootcode
+   { ipe initialized with struct \/ erase } *)
+
+  Section Bootcode.
+    Local Notation "v -' n" :=
+      (term_binop bop.bvsub v (term_val ty.wordBits [bv n]))
+      (at level 50).
+
+    Definition asn_byte_zero {Σ} (b : Term Σ ty.byteBits) : Assertion Σ :=
+      b = term_val ty.byteBits [bv 0].
+
+    Definition saved_ptr_loc {Σ} : Term Σ _ := term_val ty.Address [bv 0x4242].
+    Definition valid_flag {Σ} : Term Σ _ := term_val ty.wordBits [bv 0xAAAA].
+    Definition ipe_sig_valid_src {Σ} : Term Σ _ := term_val ty.Address [bv 0xFF88].
+    Definition ipe_struct_pointer_src {Σ} : Term Σ _ := term_val ty.Address [bv 0xFF8A].
+
+    Definition start_bootcode_start{Σ} : Term Σ _ := term_val ty.wordBits [bv 0].
+    Definition transfer_if_valid_struct_start {Σ} : Term Σ _ := term_val ty.wordBits [bv 0x6].
+    Definition check_struct_start {Σ} : Term Σ _ := term_val ty.wordBits [bv 0x14].
+    Definition evaluate_struct_start {Σ} : Term Σ _ := term_val ty.wordBits [bv 0x24].
+    Definition mass_erase_start {Σ} : Term Σ _ := term_val ty.wordBits [bv 0x38].
+    Definition end_addr {Σ} : Term Σ _ := term_val ty.wordBits [bv 0x48].
+
+    Definition asn_flag_valid {Σ} : Assertion Σ :=
+      asn_ptsto_word ipe_sig_valid_src (low valid_flag) (high valid_flag).
+
+    Definition contract_start_bootcode : BlockVerifierContract :=
+      {{
+            asn_init_pc start_bootcode_start
+
+          ∗ R10_reg ↦ saved_ptr_loc
+          ∗ asn_ptsto_word saved_ptr_loc (term_var "ptr_l") (term_var "ptr_h")
+      }}
+        [ tst_m R10
+        ; jnz [bv 5] (* check_struct *) ]
+      {{
+            R10_reg ↦ saved_ptr_loc
+          ∗ asn_ptsto_word saved_ptr_loc (term_var "ptr_l") (term_var "ptr_h")
+
+          ∗ (( (*asn_byte_zero (term_var "ptr_l")
+             ∗ asn_byte_zero (term_var "ptr_h")
+             ∗ *)asn_fin_pc transfer_if_valid_struct_start)
+            ∨ asn_fin_pc check_struct_start)
+      }}
+        with ["ptr_l" :: ty.byteBits; "ptr_h" :: ty.byteBits].
+
+    Definition contract_transfer_if_valid_struct : BlockVerifierContract :=
+      {{
+            asn_init_pc transfer_if_valid_struct_start
+
+          ∗ R10_reg ↦ saved_ptr_loc
+          ∗ R11_reg ↦ valid_flag
+          ∗ R12_reg ↦ ipe_sig_valid_src
+          ∗ R13_reg ↦ ipe_struct_pointer_src
+          ∗ asn_flag_valid
+          ∗ asn_ptsto_word ipe_struct_pointer_src
+              (term_var "struct_ptr_l") (term_var "struct_ptr_h")
+          ∗ ∃ "l", ∃ "h", asn_ptsto_word saved_ptr_loc (term_var "l") (term_var "h")
+      }}
+        [ cmp_rm R11 R12
+        ; jnz [bv 29]
+        ; mov_mm R13 R10 ]
+      {{
+            R10_reg ↦ saved_ptr_loc
+          ∗ R11_reg ↦ valid_flag
+          ∗ R12_reg ↦ ipe_sig_valid_src
+          ∗ R13_reg ↦ ipe_struct_pointer_src
+          ∗ asn_flag_valid
+          ∗ asn_ptsto_word ipe_struct_pointer_src
+              (term_var "struct_ptr_l") (term_var "struct_ptr_h")
+
+          ∗ asn_fin_pc check_struct_start
+          ∗ asn_ptsto_word saved_ptr_loc (term_var "struct_ptr_l") (term_var "struct_ptr_h")
+      }}
+        with ["struct_ptr_l" :: ty.byteBits; "struct_ptr_h" :: ty.byteBits].
+
+    Definition contract_evaluate_struct : BlockVerifierContract :=
+      {{
+           asn_init_pc evaluate_struct_start
+         ∗ asn_ipe_registers
+
+         ∗ R6_reg ↦ term_val ty.Address [bv 0x1000]
+         ∗ asn_ptsto_word (term_val ty.Address [bv 0x1000]) (term_val ty.byteBits [bv 0]) (term_val ty.byteBits [bv 0])
+
+         (* ∗ R7_reg ↦ MPUIPC0_addr *)
+         (* ∗ R8_reg ↦ MPUIPSEGB2_addr *)
+         (* ∗ R9_reg ↦ MPUIPSEGB1_addr *)
+
+         (* ∗ R6_reg ↦ term_var "struct_ptr" +' 6 *)
+
+         (* ∗ term_var "struct_ptr" = term_val ty.wordBits [bv 0x1000] *)
+
+         (* (* struct doesn't overlap MPU register file *) *)
+         (* (*    needs more preconditions to exclude overflow of struct_ptr + 6 *) *)
+         (* (* ∗ (term_unsigned (term_var "struct_ptr" +' 6) < (term_val ty.int 0x05A0%Z) *) *)
+         (* (*    ∨ term_val ty.int 0x05B0%Z <= term_unsigned (term_var "struct_ptr")) *) *)
+
+         (* ∗ asn_ptsto_word (term_var "struct_ptr" +' 4) *)
+         (*     (low (term_var "segb1")) (high (term_var "segb1")) *)
+         (* ∗ asn_ptsto_word (term_var "struct_ptr" +' 2) *)
+         (*     (low (term_var "segb2")) (high (term_var "segb2")) *)
+         (* ∗ asn_ptsto_word (term_var "struct_ptr") *)
+         (*     (low (term_var "ipectl")) (high (term_var "ipectl")) *)
+      }}
+        [ mov_rm R6 R6          (* fix offsets *)
+          (* mov_im R6 (bv.of_Z (-2)%Z) R9 *)
+        (* ; mov_im R6 (bv.of_Z (-4)%Z) R8 *)
+        (* ; mov_im R6 (bv.of_Z (-6)%Z) R7 *)
+        (* ; jump JMP [bv (* 0x08 *) 0x10] *) (* end *)]
+      {{ ⊥
+         (*   (* asn_fin_pc end_addr *) *)
+         (*   PC_reg         ↦ end_addr *)
+         (* ∗ MPUIPC0_reg    ↦ term_var "ipectl" *)
+         (* ∗ MPUIPSEGB1_reg ↦ term_var "segb1" *)
+         (* ∗ MPUIPSEGB2_reg ↦ term_var "segb2" *)
+
+         (* ∗ R6_reg ↦ term_var "struct_ptr" +' 6 *)
+         (* ∗ R7_reg ↦ MPUIPC0_addr *)
+         (* ∗ R8_reg ↦ MPUIPSEGB2_addr *)
+         (* ∗ R9_reg ↦ MPUIPSEGB1_addr *)
+      }}
+        with ["ipectl" :: ty.wordBits; "segb1" :: ty.wordBits; "segb2" :: ty.wordBits; "struct_ptr" :: ty.Address].
+
+    Lemma valid_start_bootcode : ValidBlockVerifierContract contract_start_bootcode.
+    Proof. vm_compute. Set Printing Depth 200. Unset Printing 
+           (* 0xe/0x4 = 0x14 *)
+           symbolic_simpl.
+           repeat split; try lia.
+           intuition.
+           auto 10 with *.
+           repeat split.
+
+           vm_compute. Set Printing Depth 200.
+    Qed.
+
+    (* Lemma valid_transfer_if_valid_struct : ValidBlockVerifierContract contract_transfer_if_valid_struct. *)
+    (* Proof. vm_compute.  *)
+
+    Lemma valid_evaluate_struct : ValidBlockVerifierContractWithExplicitIPE contract_evaluate_struct.
+    Proof.
+      symbolic_simpl.
+      repeat right.
+      rewrite H. unfold bv.add. vm_compute.
+      intuition; discriminate.
+    Qed.
+
+    (* TODO is check_byte_access's contract good enough? *)
+
+  End Bootcode.
 End Examples.
+
+(*
+{|
+debug_consume_chunk_pathcondition :=
+[formula_relop
+bop.eq
+(term_var
+"struct_ptr" +' 0x4)
+(term_binop
+bop.bvand
+(term_var
+"struct_ptr" +' 0x4)
+(term_val
+ty.Address
+[bv 0xfffe]));
+formula_relop
+bop.eq
+(term_var
+"struct_ptr" +' 0x2)
+(term_binop
+bop.bvand
+(term_var
+"struct_ptr" +' 0x2)
+(term_val
+ty.Address
+[bv 0xfffe]));
+formula_relop
+bop.eq
+(term_var
+"struct_ptr")
+(term_binop
+bop.bvand
+(term_var
+"struct_ptr")
+(term_val
+ty.Address
+[bv 0xfffe]));
+formula_relop
+bop.eq
+(term_var "bh.1" @
+term_var "bl.1")
+(term_val
+ty.Address
+[bv 0xfffe]);
+formula_relop
+bop.eq
+(term_binop
+bop.bvadd
+(term_var
+"struct_ptr")
+(term_var "bh.1" @
+term_var "bl.1") +'
+0x6)
+(term_binop
+bop.bvand
+(term_binop
+bop.bvadd
+(term_var
+"struct_ptr")
+(term_var "bh.1" @
+term_var "bl.1") +'
+0x6)
+(term_val
+ty.Address
+[bv 0xfffe]));
+formula_relop
+bop.eq
+(term_binop
+bop.bvadd
+(term_var
+"struct_ptr")
+(term_var "bh.1" @
+term_var "bl.1") +'
+0x6)
+(term_var
+"struct_ptr" +' 0x4);
+formula_relop
+bop.eq
+(term_binop
+bop.bvor
+(term_binop
+bop.bvadd
+(term_var
+"struct_ptr")
+(term_var "bh.1" @
+term_var "bl.1") +'
+0x6)
+(term_val
+ty.Address [bv 0x1]))
+(term_binop
+bop.bvor
+(term_var
+"struct_ptr" +' 0x4)
+(term_val
+ty.Address [bv 0x1]));
+formula_relop
+bop.le
+(term_val ty.int
+1456%Z)
+(term_unsigned
+(term_binop
+bop.bvadd
+(term_var
+"struct_ptr")
+(term_var "bh.1" @
+term_var "bl.1") +'
+0x6));
+formula_relop
+bop.le
+(term_val ty.int
+1456%Z)
+(term_unsigned
+(term_binop
+bop.bvor
+(term_binop
+bop.bvadd
+(term_var
+"struct_ptr")
+(term_var "bh.1" @
+term_var "bl.1") +'
+0x6)
+(term_val
+ty.Address [bv 0x1])))];
+debug_consume_chunk_heap :=
+[chunk_ptsreg
+R9_reg
+(term_vector_subrange
+0 8
+(term_var "segb1") @
+term_vector_subrange
+8 8
+(term_var "segb1"));
+chunk_ptsreg
+LastInstructionFetch
+(term_val
+(ty.union Uwordbyte)
+(Word [bv 0x0]));
+chunk_ptsreg
+MPUIPSEGB2_reg
+(term_var "segb2.2");
+chunk_ptsreg
+MPUIPSEGB1_reg
+(term_var "segb1.2");
+chunk_ptsreg
+MPUIPC0_reg
+(term_var
+"ipectl.2");
+chunk_user ptstomem
+[term_binop
+bop.bvor
+(term_binop
+bop.bvadd
+(term_var
+"struct_ptr")
+(term_var "bh.1" @
+term_var "bl.1") +'
+0x6)
+(term_val
+ty.Address [bv 0x1]);
+term_vector_subrange
+0 8
+(term_var "segb1")];
+chunk_user ptstomem
+[term_binop
+bop.bvadd
+(term_var
+"struct_ptr")
+(term_var "bh.1" @
+term_var "bl.1") +'
+0x6;
+term_vector_subrange
+8 8
+(term_var "segb1")];
+chunk_user
+ptstoinstr
+[term_val
+ty.Address
+[bv 0x26];
+term_union
+Uinstr_or_data Kd
+(term_var "bh.1" @
+term_var "bl.1")];
+chunk_ptsreg R6_reg
+(term_var
+"struct_ptr" +' 0x6);
+chunk_user
+ptstoinstr
+[term_val
+ty.Address
+[bv 0x24];
+term_union
+Uinstr_or_data Kd
+(term_var "bh" @
+term_var "bl")];
+chunk_user
+encodes_instr
+[term_var "bh" @
+term_var "bl";
+term_val
+(ty.union Uast)
+(DOUBLEOP MOV
+WORD_INSTRUCTION R6
+INDEXED_MODE R9
+REGISTER_MODE)];
+chunk_user ptstomem
+[term_binop
+bop.bvor
+(term_var
+"struct_ptr")
+(term_val
+ty.Address [bv 0x1]);
+term_vector_subrange
+0 8
+(term_var "ipectl")];
+chunk_user ptstomem
+[term_var
+"struct_ptr";
+term_vector_subrange
+8 8
+(term_var "ipectl")];
+chunk_user ptstomem
+[term_binop
+bop.bvor
+(term_var
+"struct_ptr" +' 0x2)
+(term_val
+ty.Address [bv 0x1]);
+term_vector_subrange
+0 8
+(term_var "segb2")];
+chunk_user ptstomem
+[term_var
+"struct_ptr" +' 0x2;
+term_vector_subrange
+8 8
+(term_var "segb2")];
+chunk_ptsreg R8_reg
+(term_val
+ty.Address
+[bv 0x5ac]);
+chunk_ptsreg R7_reg
+(term_val
+ty.Address
+[bv 0x5aa]);
+chunk_ptsreg
+MPUIPSEGB2_reg
+(term_var "segb2.1");
+chunk_ptsreg
+MPUIPSEGB1_reg
+(term_var "segb1.1");
+chunk_ptsreg
+MPUIPC0_reg
+(term_var
+"ipectl.1")]%list;
+debug_consume_chunk_chunk :=
+chunk_user
+ptstoinstr
+[term_val
+ty.Address
+[bv 0x24];
+term_val
+(ty.union
+Uinstr_or_data)
+(I
+(DOUBLEOP MOV
+WORD_INSTRUCTION R6
+INDEXED_MODE R9
+REGISTER_MODE))]
+|}
+
+ *)
